examples/atuin/schema.sql
@@ -1,12 +1,3 @@
-CREATE TABLE _sqlx_migrations (
-    version BIGINT PRIMARY KEY,
-    description TEXT NOT NULL,
-    installed_on TIMESTAMP NOT NULL DEFAULT CURRENT_TIMESTAMP,
-    success BOOLEAN NOT NULL,
-    checksum BLOB NOT NULL,
-    execution_time BIGINT NOT NULL
-);
-
 CREATE TABLE history (
 	id text primary key,
 	timestamp integer not null,
